src/program_proof/lockservice/rpc_proof.v
@@ -7,6 +7,8 @@ From Perennial.program_proof Require Import proof_prelude.
 From Perennial.program_proof.lockservice Require Import lockservice_nocrash common_proof.
 From Perennial.program_proof.lockservice Require Export rpc.
 From Goose.github_com.mit_pdos.lockservice Require Import grove_common.
+From Perennial.goose_lang.lib.slice Require Import typed_slice.
+From Perennial.program_proof Require Import marshal_proof.
 
 Section rpc_proof.
 Context `{!heapG Σ}.
@@ -33,7 +35,7 @@ Proof.
 Defined.
 
 Definition read_request (args_ptr:loc) (req : RPCRequestID) (args:RPCValsC) : iProp Σ :=
-    "#HSeqPositive" ∷ ⌜int.nat req.(Req_Seq) > 0⌝ ∗
+    "%HSeqPositive" ∷ ⌜int.nat req.(Req_Seq) > 0⌝ ∗
     "#HArgsOwnArgs" ∷ readonly (args_ptr ↦[RPCRequest.S :: "Args"] (into_val.to_val args)) ∗
     "#HArgsOwnCID" ∷ readonly (args_ptr ↦[RPCRequest.S :: "CID"] #req.(Req_CID)) ∗
     "#HArgsOwnSeq" ∷ readonly (args_ptr ↦[RPCRequest.S :: "Seq"] #req.(Req_Seq))
@@ -275,6 +277,162 @@ Proof.
   }
 Qed.
 
+Definition reqEncoded (req:RPCRequestID) (args:RPCValsC) (bs:list u8) : Prop :=
+  int.nat req.(Req_Seq) > 0 ∧
+  has_encoding bs [EncUInt64 req.(Req_CID);
+                   EncUInt64 req.(Req_Seq);
+                   EncUInt64 args.(U64_1);
+                   EncUInt64 args.(U64_2)].
+
+Theorem wp_rpcReqEncode (req_ptr:loc) (req:RPCRequestID) (args:RPCValsC) :
+  {{{
+    read_request req_ptr req args
+  }}}
+    rpcReqEncode #req_ptr
+  {{{
+    s (bs:list u8), RET (slice_val s);
+    is_slice s u8T 1%Qp bs ∗
+    ⌜reqEncoded req args bs⌝
+  }}}.
+Proof.
+  iIntros (Φ) "#Hreq HΦ".
+  iNamed "Hreq".
+  wp_call.
+  wp_apply wp_new_enc.
+  iIntros (e) "He".
+  wp_loadField.
+  wp_apply (wp_Enc__PutInt with "He").
+  { admit. }
+  iIntros "He".
+  wp_loadField.
+  wp_apply (wp_Enc__PutInt with "He").
+  { admit. }
+  iIntros "He".
+  wp_loadField.
+  wp_apply (wp_Enc__PutInt with "He").
+  { admit. }
+  iIntros "He".
+  wp_loadField.
+  wp_apply (wp_Enc__PutInt with "He").
+  { admit. }
+  iIntros "He".
+  wp_apply (wp_Enc__Finish with "He").
+  iIntros (s bs) "(%Hhasenc & %Hlen & Hs)".
+  wp_pures.
+  iApply "HΦ".
+  iFrame "Hs".
+  iPureIntro. rewrite /reqEncoded.
+  simpl in Hhasenc. eauto.
+Admitted.
+
+Theorem wp_rpcReqDecode (s:Slice.t) (reqptr:loc) (bs:list u8) (req:RPCRequestID) (args:RPCValsC) q :
+  {{{
+    is_slice_small s u8T q bs ∗
+    ⌜reqEncoded req args bs⌝ ∗
+    reqptr ↦[struct.t RPCRequest.S] (#0, (#0, (#0, (#0, #()), #())))
+  }}}
+    rpcReqDecode (slice_val s) #reqptr
+  {{{
+    RET #();
+    read_request reqptr req args
+  }}}.
+Proof.
+  iIntros (Φ) "(Hs & %Henc & Hreq) HΦ".
+  iDestruct (struct_fields_split with "Hreq") as "Hreq". iNamed "Hreq".
+  wp_call.
+  wp_apply (wp_new_dec with "Hs").
+  { eapply Henc. }
+  iIntros (d) "Hd".
+  wp_apply (wp_Dec__GetInt with "Hd"). iIntros "Hd".
+  wp_storeField.
+  wp_apply (wp_Dec__GetInt with "Hd"). iIntros "Hd".
+  wp_storeField.
+  wp_apply (wp_Dec__GetInt with "Hd"). iIntros "Hd".
+  wp_apply (wp_struct_fieldRef_mapsto with "Args"); first done.
+  iIntros (fl) "[%Hfl Args]".
+  wp_apply (wp_storeField_struct with "Args"); first auto.
+  iIntros "Args".
+  rewrite Hfl; clear Hfl fl.
+  wp_apply (wp_Dec__GetInt with "Hd"). iIntros "Hd".
+  wp_apply (wp_struct_fieldRef_mapsto with "Args"); first done.
+  iIntros (fl) "[%Hfl Args]".
+  wp_apply (wp_storeField_struct with "Args"); first auto.
+  iIntros "Args".
+  rewrite Hfl; clear Hfl fl.
+  rewrite /=.
+  iMod (readonly_alloc_1 with "CID") as "#CID".
+  iMod (readonly_alloc_1 with "Seq") as "#Seq".
+  iMod (readonly_alloc_1 with "Args") as "#Args".
+  wp_pures.
+  iApply "HΦ".
+  destruct Henc as [Hseqpos Henc].
+  iSplit; eauto.
+Qed.
+
+Definition replyEncoded (r:RPCReply) (bs:list u8) : Prop :=
+  has_encoding bs [EncBool r.(Rep_Stale);
+                   EncUInt64 r.(Rep_Ret)].
+
+Theorem wp_rpcReplyEncode (reply_ptr:loc) (reply:RPCReply) :
+  {{{
+    own_reply reply_ptr reply
+  }}}
+    rpcReplyEncode #reply_ptr
+  {{{
+    s (bs:list u8), RET (slice_val s);
+    is_slice s u8T 1%Qp bs ∗
+    ⌜replyEncoded reply bs⌝
+  }}}.
+Proof.
+  iIntros (Φ) "Hreply HΦ".
+  iNamed "Hreply".
+  wp_call.
+  wp_apply wp_new_enc.
+  iIntros (e) "He".
+  wp_loadField.
+  wp_apply (wp_Enc__PutBool with "He").
+  { admit. }
+  iIntros "He".
+  wp_loadField.
+  wp_apply (wp_Enc__PutInt with "He").
+  { admit. }
+  iIntros "He".
+  wp_apply (wp_Enc__Finish with "He").
+  iIntros (s bs) "(%Hhasenc & %Hlen & Hs)".
+  wp_pures.
+  iApply "HΦ".
+  iFrame "Hs".
+  iPureIntro. rewrite /replyEncoded.
+  simpl in Hhasenc. eauto.
+Admitted.
+
+Theorem wp_rpcReplyDecode (s:Slice.t) (reply_ptr:loc) (bs:list u8) (reply:RPCReply) q (v0 : bool) (v1 : u64) :
+  {{{
+    is_slice_small s u8T q bs ∗
+    ⌜replyEncoded reply bs⌝ ∗
+    reply_ptr ↦[struct.t RPCReply.S] (#v0, (#v1, #()))
+  }}}
+    rpcReplyDecode (slice_val s) #reply_ptr
+  {{{
+    RET #();
+    own_reply reply_ptr reply
+  }}}.
+Proof.
+  iIntros (Φ) "(Hs & %Henc & Hreply) HΦ".
+  iDestruct (struct_fields_split with "Hreply") as "Hreply". iNamed "Hreply".
+  wp_call.
+  wp_apply (wp_new_dec with "Hs").
+  { eapply Henc. }
+  iIntros (d) "Hd".
+  wp_apply (wp_Dec__GetBool with "Hd"). iIntros "Hd".
+  wp_storeField.
+  wp_apply (wp_Dec__GetInt with "Hd"). iIntros "Hd".
+  wp_storeField.
+  wp_pures.
+  iApply "HΦ".
+  iSplitL "Stale"; iFrame.
+Qed.
+
 Lemma RemoteProcedureCall_spec (req_ptr reply_ptr:loc) (req:RPCRequestID)
                                args (reply:Reply64) (host:u64) (rpcid:u64)
                                PreCond PostCond γrpc γPost :
@@ -300,8 +458,17 @@ Proof.
   simpl.
   wp_let.
   wp_let.
-  wp_apply wp_fork.
+  wp_let.
+  wp_apply (wp_rpcReqEncode with "Hargs").
+  iIntros (reqSlice reqBs) "[HreqSlice %Hreqenc]".
+  iDestruct (is_slice_to_small with "HreqSlice") as "HreqSlice".
+
+Opaque is_slice_small.
+  iDestruct "HreqSlice" as "[HreqSlice0 HreqSlice1]".
+
+  wp_apply (wp_fork with "[HreqSlice1]").
   {
+    iModIntro.
     wp_apply (wp_allocStruct); first by eauto.
     iIntros (l) "Hl".
     iDestruct (struct_fields_split with "Hl") as "[HStale HRet]".
@@ -310,17 +477,31 @@ Proof.
     (* Set up loop invariant *)
     iAssert (∃ reply, (own_reply l reply))%I with "[Stale Ret]" as "Hreply".
     { iExists {| Rep_Stale:=false; Rep_Ret:=_ |}. iFrame. }
+    iAssert (∃ q, is_slice_small reqSlice u8T q reqBs)%I with "[HreqSlice1]" as "HreqSlice1".
+    { iExists _; iFrame. }
     wp_forBreak. wp_pures.
     iDestruct "Hreply" as (reply') "Hreply".
 
     iNamed "Hspec".
     wp_apply (wp_GetServer with "[$Hhost]"); eauto.
     wp_let.
-    wp_apply ("Hhandler" with "[-]").
+
+    wp_apply (wp_allocStruct); first by eauto.
+    iIntros (sreqptr) "Hsreqptr".
+    wp_pures.
+
+    iDestruct "HreqSlice1" as (q) "HreqSlice1".
+    iDestruct "HreqSlice1" as "[HreqSlice10 HreqSlice11]".
+    wp_apply (wp_rpcReqDecode with "[$HreqSlice10 $Hsreqptr]"); eauto.
+    iIntros "Hargs_server".
+
+    wp_apply ("Hhandler" with "[-HreqSlice11]").
     { iFrame "#∗". }
     iIntros "fPost".
     wp_seq. iLeft. iSplitR; first done.
     iDestruct "fPost" as (reply'') "[Hreply fPost]".
+    iSplitL "Hreply".
+    { iExists _. done. }
     iExists _. done.
   }
   wp_seq.
@@ -332,8 +513,44 @@ Proof.
     iNamed "Hspec".
     wp_apply (wp_GetServer with "[$Hhost]"); eauto.
     wp_let.
-    wp_apply ("Hhandler" with "[$Hreply]"); eauto; try iFrame "#".
-    iDestruct 1 as (reply') "[Hreply fPost]".
+
+    wp_apply (wp_allocStruct); first by eauto.
+    iIntros (sreqptr) "Hsreqptr".
+    wp_pures.
+
+    wp_apply (wp_rpcReqDecode with "[$HreqSlice0 $Hsreqptr]"); eauto.
+    iIntros "Hargs_server".
+
+    wp_apply (wp_allocStruct); first by eauto.
+    iIntros (sreplyptr) "Hsreplyptr".
+    wp_pures.
+
+    wp_apply ("Hhandler" with "[Hsreplyptr]").
+    { iFrame "#".
+      replace (#false) with (#(@Build_RPCReply u64 false (U64 0)).(Rep_Stale)) by reflexivity.
+      iDestruct (struct_fields_split with "Hsreplyptr") as "Hsreplyptr". iNamed "Hsreplyptr".
+      iSplitL "Stale". { iFrame. }
+      iFrame.
+    }
+    iDestruct 1 as (reply') "[Hsreplyptr fPost]".
+    wp_pures.
+
+    wp_apply (wp_rpcReplyEncode with "Hsreplyptr").
+    iIntros (reply_s reply_bs) "[Hreply_s %Hreply_bs]".
+
+    iDestruct (is_slice_to_small with "Hreply_s") as "Hreply_s".
+
+    wp_pures.
+    wp_apply (wp_rpcReplyDecode with "[$Hreply_s Hreply]").
+    { iSplit; eauto.
+      iApply struct_fields_split.
+      rewrite /struct_fields /struct.struct_big_fields_rec /=.
+      iNamed "Hreply".
+      iSplitL "HReplyOwnStale"; iFrame. done.
+    }
+    iIntros "Hreplydec".
+    wp_pures.
+
     iApply "Hpost".
     iFrame.
     iExists _; iFrame.
